<?xml version="1.0"?>
<rdf:RDF xmlns="http://vocab.linkeddata.es/datosabiertos/def/medio-ambiente/contaminacion-acustica#"
     xml:base="http://vocab.linkeddata.es/datosabiertos/def/medio-ambiente/contaminacion-acustica"
     xmlns:rdf="http://www.w3.org/1999/02/22-rdf-syntax-ns#"
     xmlns:terms="http://purl.org/dc/terms/"
     xmlns:owl="http://www.w3.org/2002/07/owl#"
     xmlns:ns="http://creativecommons.org/ns#"
     xmlns:xml="http://www.w3.org/XML/1998/namespace"
     xmlns:noise="http://vocab.linkeddata.es/datosabiertos/def/medio-ambiente/contaminacion-acustica#"
     xmlns:xsd="http://www.w3.org/2001/XMLSchema#"
     xmlns:wgs84_pos="http://www.w3.org/2003/01/geo/wgs84_pos#"
     xmlns:rdfs="http://www.w3.org/2000/01/rdf-schema#"
     xmlns:vann="http://purl.org/vocab/vann/"
     xmlns:foaf="http://xmlns.com/foaf/0.1/"
     xmlns:dc="http://purl.org/dc/elements/1.1/">
    <owl:Ontology rdf:about="http://vocab.linkeddata.es/datosabiertos/def/medio-ambiente/contaminacion-acustica">
        <owl:imports rdf:resource="http://purl.oclc.org/NET/ssnx/ssn"/>
        <owl:imports rdf:resource="http://www.w3.org/2006/time"/>
        <dc:title xml:lang="es">Contaminación Acústica</dc:title>
        <dc:description xml:lang="es">Este vocabulario extiende la W3C Semantic Sensor Network Ontology (SSN) con propiedades para representar los datos de la contaminación acústica. También se extiende la OWL Ontology of Time (OWL-Time)  para representar el tiempo y la WGS84 Geo Positioning para representar la posición en el espacio a través de la longitud, latitud y altitud</dc:description>
        <dc:contributor xml:lang="es">Mariano Fernández López</dc:contributor>
        <dc:contributor xml:lang="es">María Poveda Villalón (Ontology Engineering Group)</dc:contributor>
        <dc:contributor xml:lang="es">Oscar Corcho García (Ontology Engineering Group)</dc:contributor>
        <dc:rights>Creative Commons Attribution 4.0 International (CC BY 4.0)</dc:rights>
        <ns:license>http://creativecommons.org/licenses/by/4.0/</ns:license>
        <dc:creator xml:lang="es">Paola Espinoza Arias (Ontology Engineering Group)</dc:creator>
    </owl:Ontology>
    


    <!-- 
    ///////////////////////////////////////////////////////////////////////////////////////
    //
    // Annotation properties
    //
    ///////////////////////////////////////////////////////////////////////////////////////
     -->

    


    <!-- http://purl.org/dc/elements/1.1/contributor -->

    <owl:AnnotationProperty rdf:about="http://purl.org/dc/elements/1.1/contributor"/>
    


    <!-- http://purl.org/dc/elements/1.1/description -->

    <owl:AnnotationProperty rdf:about="http://purl.org/dc/elements/1.1/description"/>
    


    <!-- http://purl.org/vocab/vann/preferredNamespacePrefix -->

    <owl:AnnotationProperty rdf:about="http://purl.org/vocab/vann/preferredNamespacePrefix"/>
    


    <!-- http://purl.org/vocab/vann/preferredNamespaceUri -->

    <owl:AnnotationProperty rdf:about="http://purl.org/vocab/vann/preferredNamespaceUri"/>
    


    <!-- http://www.w3.org/1999/02/22-rdf-syntax-ns#value -->

    <owl:AnnotationProperty rdf:about="http://www.w3.org/1999/02/22-rdf-syntax-ns#value"/>
    


    <!-- http://www.w3.org/2003/01/geo/wgs84_pos#location -->

    <owl:AnnotationProperty rdf:about="http://www.w3.org/2003/01/geo/wgs84_pos#location">
        <rdfs:subPropertyOf rdf:resource="http://xmlns.com/foaf/0.1/based_near"/>
        <rdfs:range rdf:resource="http://www.w3.org/2003/01/geo/wgs84_pos#SpatialThing"/>
    </owl:AnnotationProperty>
    


    <!-- http://xmlns.com/foaf/0.1/based_near -->

    <owl:AnnotationProperty rdf:about="http://xmlns.com/foaf/0.1/based_near"/>
    


    <!-- 
    ///////////////////////////////////////////////////////////////////////////////////////
    //
    // Object Properties
    //
    ///////////////////////////////////////////////////////////////////////////////////////
     -->

    


    <!-- http://purl.oclc.org/NET/ssnx/ssn#observationSamplingTime -->

    <rdf:Description rdf:about="http://purl.oclc.org/NET/ssnx/ssn#observationSamplingTime">
        <rdfs:domain rdf:resource="http://purl.oclc.org/NET/ssnx/ssn#ObservationValue"/>
        <rdfs:range rdf:resource="http://www.w3.org/2006/time#TemporalEntity"/>
    </rdf:Description>
    


    <!-- http://vocab.linkeddata.es/datosabiertos/def/medio-ambiente/contaminacion-acustica#belongsToSensorClass -->

    <owl:ObjectProperty rdf:about="http://vocab.linkeddata.es/datosabiertos/def/medio-ambiente/contaminacion-acustica#belongsToSensorClass">
        <rdfs:domain rdf:resource="http://vocab.linkeddata.es/datosabiertos/def/medio-ambiente/contaminacion-acustica#NoiseSensor"/>
        <rdfs:range rdf:resource="http://www.w3.org/2004/02/skos/core#Concept"/>
    </owl:ObjectProperty>
    


    <!-- http://vocab.linkeddata.es/datosabiertos/def/medio-ambiente/contaminacion-acustica#hasUnitOfMeasure -->

    <owl:ObjectProperty rdf:about="http://vocab.linkeddata.es/datosabiertos/def/medio-ambiente/contaminacion-acustica#hasUnitOfMeasure">
        <rdfs:domain rdf:resource="http://purl.oclc.org/NET/ssnx/ssn#SensorOutput"/>
        <rdfs:range rdf:resource="http://www.wurvoc.org/vocabularies/om-1.8/Unit_of_measure"/>
        <rdfs:label xml:lang="en">has unit of measure</rdfs:label>
    </owl:ObjectProperty>
    


    <!-- http://vocab.linkeddata.es/datosabiertos/def/medio-ambiente/contaminacion-acustica#isWeightingWith -->

    <owl:ObjectProperty rdf:about="http://vocab.linkeddata.es/datosabiertos/def/medio-ambiente/contaminacion-acustica#isWeightingWith">
        <rdfs:domain rdf:resource="http://purl.oclc.org/NET/ssnx/ssn#ObservationValue"/>
        <rdfs:range rdf:resource="http://vocab.linkeddata.es/datosabiertos/def/medio-ambiente/contaminacion-acustica#Weighting"/>
        <rdfs:comment xml:lang="es">La medida que realiza el Sensor de Ruido tiene una ponderación frecuencial. Puede ser sin poderación (Z), ponderación A o C</rdfs:comment>
        <rdfs:label xml:lang="es">es ponderado con</rdfs:label>
        <rdfs:label xml:lang="en">is weightin with</rdfs:label>
    </owl:ObjectProperty>
    


    <!-- http://www.w3.org/2003/01/geo/wgs84_pos#alt -->

    <owl:ObjectProperty rdf:about="http://www.w3.org/2003/01/geo/wgs84_pos#alt">
        <rdfs:domain rdf:resource="http://www.w3.org/2003/01/geo/wgs84_pos#SpatialThing"/>
        <rdfs:comment>The WGS84 altitude of a SpatialThing (decimal meters 
above the local reference ellipsoid).</rdfs:comment>
        <rdfs:label xml:lang="es">altitud</rdfs:label>
        <rdfs:label>altitude</rdfs:label>
    </owl:ObjectProperty>
    


    <!-- http://www.w3.org/2003/01/geo/wgs84_pos#lat -->

    <owl:ObjectProperty rdf:about="http://www.w3.org/2003/01/geo/wgs84_pos#lat">
        <rdfs:domain rdf:resource="http://www.w3.org/2003/01/geo/wgs84_pos#SpatialThing"/>
        <rdfs:comment>The WGS84 latitude of a SpatialThing (decimal degrees).</rdfs:comment>
        <rdfs:label xml:lang="es">latitud</rdfs:label>
        <rdfs:label>latitude</rdfs:label>
    </owl:ObjectProperty>
    


    <!-- http://www.w3.org/2003/01/geo/wgs84_pos#location -->

    <owl:ObjectProperty rdf:about="http://www.w3.org/2003/01/geo/wgs84_pos#location">
        <rdfs:domain rdf:resource="http://purl.oclc.org/NET/ssnx/ssn#SensingDevice"/>
    </owl:ObjectProperty>
    


    <!-- http://www.w3.org/2003/01/geo/wgs84_pos#long -->

    <owl:ObjectProperty rdf:about="http://www.w3.org/2003/01/geo/wgs84_pos#long">
        <rdfs:domain rdf:resource="http://www.w3.org/2003/01/geo/wgs84_pos#SpatialThing"/>
        <rdfs:comment>The WGS84 longitude of a SpatialThing (decimal degrees).</rdfs:comment>
        <rdfs:label xml:lang="es">longitud</rdfs:label>
        <rdfs:label>longitude</rdfs:label>
    </owl:ObjectProperty>
    


    <!-- 
    ///////////////////////////////////////////////////////////////////////////////////////
    //
    // Data properties
    //
    ///////////////////////////////////////////////////////////////////////////////////////
     -->

    


    <!-- http://vocab.linkeddata.es/datosabiertos/def/medio-ambiente/contaminacion-acustica#lastCalibrationDate -->

    <owl:DatatypeProperty rdf:about="http://vocab.linkeddata.es/datosabiertos/def/medio-ambiente/contaminacion-acustica#lastCalibrationDate">
        <rdfs:domain rdf:resource="http://vocab.linkeddata.es/datosabiertos/def/medio-ambiente/contaminacion-acustica#NoiseSensor"/>
        <rdfs:range rdf:resource="http://www.w3.org/2001/XMLSchema#dateTime"/>
        <rdfs:comment xml:lang="es">Última fecha de calibración del sensor.  La calibración es un proceso periódico realizado a los sensores acústicos para verificar su correcto funcionamiento en sus distintos modos de trabajo.</rdfs:comment>
        <rdfs:label xml:lang="en">last calibration date</rdfs:label>
        <rdfs:label xml:lang="es">última fecha de calibración</rdfs:label>
    </owl:DatatypeProperty>
    


    <!-- 
    ///////////////////////////////////////////////////////////////////////////////////////
    //
    // Classes
    //
    ///////////////////////////////////////////////////////////////////////////////////////
     -->

    


    <!-- http://vocab.linkeddata.es/datosabiertos/def/medio-ambiente/contaminacion-acustica#AverageNoiseLevel -->

    <owl:Class rdf:about="http://vocab.linkeddata.es/datosabiertos/def/medio-ambiente/contaminacion-acustica#AverageNoiseLevel">
        <rdfs:subClassOf rdf:resource="http://vocab.linkeddata.es/datosabiertos/def/medio-ambiente/contaminacion-acustica#NoiseLevel"/>
        <rdfs:comment xml:lang="es">Nivel medio de ruido que ha sido medido por el sensor.</rdfs:comment>
        <rdfs:label xml:lang="en">Average Noise Level</rdfs:label>
        <rdfs:label xml:lang="es">Nivel Medio de Ruido</rdfs:label>
    </owl:Class>
    


    <!-- http://vocab.linkeddata.es/datosabiertos/def/medio-ambiente/contaminacion-acustica#NoiseLevel -->

    <owl:Class rdf:about="http://vocab.linkeddata.es/datosabiertos/def/medio-ambiente/contaminacion-acustica#NoiseLevel">
        <rdfs:subClassOf rdf:resource="http://purl.oclc.org/NET/ssnx/ssn#Property"/>
        <rdfs:comment xml:lang="es">Nivel de ruido que ha sido medido por el sensor. Se mide en Decibelios (dB)</rdfs:comment>
        <rdfs:label xml:lang="es">Nivel de Ruido</rdfs:label>
        <rdfs:label xml:lang="en">Noise Level</rdfs:label>
    </owl:Class>
    


    <!-- http://vocab.linkeddata.es/datosabiertos/def/medio-ambiente/contaminacion-acustica#NoiseSensor -->

    <owl:Class rdf:about="http://vocab.linkeddata.es/datosabiertos/def/medio-ambiente/contaminacion-acustica#NoiseSensor">
        <rdfs:subClassOf rdf:resource="http://purl.oclc.org/NET/ssnx/ssn#SensingDevice"/>
        <rdfs:comment xml:lang="es">Mide el nivel de ruido</rdfs:comment>
        <rdfs:label xml:lang="en">Noise Sensor</rdfs:label>
        <rdfs:label xml:lang="es">Sensor de Ruido</rdfs:label>
    </owl:Class>
    


    <!-- http://vocab.linkeddata.es/datosabiertos/def/medio-ambiente/contaminacion-acustica#PercentilNoiseLevel -->

    <owl:Class rdf:about="http://vocab.linkeddata.es/datosabiertos/def/medio-ambiente/contaminacion-acustica#PercentilNoiseLevel">
        <rdfs:subClassOf rdf:resource="http://vocab.linkeddata.es/datosabiertos/def/medio-ambiente/contaminacion-acustica#NoiseLevel"/>
        <rdfs:comment xml:lang="es">Nivel de presión sonora ponderado en frecuencia y ponderado en el tiempo superado el N% de tiempo del intervalo considerado</rdfs:comment>
        <rdfs:label xml:lang="es">Nivel de Ruido en Percentiles</rdfs:label>
        <rdfs:label xml:lang="en">Percentil Noise Level</rdfs:label>
        <rdfs:seeAlso xml:lang="es">AENOR: UNE-ISO 1996-1</rdfs:seeAlso>
    </owl:Class>
    


    <!-- http://vocab.linkeddata.es/datosabiertos/def/medio-ambiente/contaminacion-acustica#Weighting -->

    <owl:Class rdf:about="http://vocab.linkeddata.es/datosabiertos/def/medio-ambiente/contaminacion-acustica#Weighting">
        <rdfs:subClassOf rdf:resource="http://www.loa-cnr.it/ontologies/DUL.owl#Method"/>
        <rdfs:comment xml:lang="es">La medida que realiza el Sensor de Ruido tiene una ponderación frecuencial. Puede ser sin poderación (Z), ponderación A o C</rdfs:comment>
        <rdfs:label xml:lang="es">Ponderación</rdfs:label>
        <rdfs:label xml:lang="en">Weighting</rdfs:label>
    </owl:Class>
    


    <!-- http://www.w3.org/2003/01/geo/wgs84_pos#Point -->

    <owl:Class rdf:about="http://www.w3.org/2003/01/geo/wgs84_pos#Point">
        <rdfs:subClassOf rdf:resource="http://www.w3.org/2003/01/geo/wgs84_pos#SpatialThing"/>
        <rdfs:comment> 
Uniquely identified by lat/long/alt. i.e.

spaciallyIntersects(P1, P2) :- lat(P1, LAT), long(P1, LONG), alt(P1, ALT),
  lat(P2, LAT), long(P2, LONG), alt(P2, ALT).

sameThing(P1, P2) :- type(P1, Point), type(P2, Point), spaciallyIntersects(P1, P2).
  </rdfs:comment>
        <rdfs:comment>A point, typically described using a coordinate system relative to Earth, such as WGS84.
  </rdfs:comment>
        <rdfs:label>point</rdfs:label>
    </owl:Class>
    


    <!-- http://www.w3.org/2003/01/geo/wgs84_pos#SpatialThing -->

    <owl:Class rdf:about="http://www.w3.org/2003/01/geo/wgs84_pos#SpatialThing">
        <rdfs:comment>Anything with spatial extent, i.e. size, shape, or position.
 e.g. people, places, bowling balls, as well as abstract areas like cubes.
</rdfs:comment>
        <rdfs:label>SpatialThing</rdfs:label>
    </owl:Class>
    


    <!-- http://www.w3.org/2004/02/skos/core#Concept -->

    <owl:Class rdf:about="http://www.w3.org/2004/02/skos/core#Concept"/>
    


    <!-- http://www.wurvoc.org/vocabularies/om-1.8/Unit_of_measure -->

    <owl:Class rdf:about="http://www.wurvoc.org/vocabularies/om-1.8/Unit_of_measure">
        <rdfs:comment xml:lang="en">A unit of measure is a definite magnitude of a quantity, defined and adopted by convention and/or by law. It is used as a standard for measurement of the same quantity, where any other value of the quantity can be expressed as a simple multiple of the unit of measure. For example, length is a quantity; the metre is a unit of length that represents a definite predetermined length. When we say 10 metre (or 10 m), we actually mean 10 times the definite predetermined length called &quot;metre&quot;. (definition taken from om ontology)</rdfs:comment>
        <rdfs:comment xml:lang="es">Una unidad de medida es una magnitud definida de una cantidad, definida y adoptada por convención y / o por ley. Se utiliza como estándar para medir la misma cantidad, donde cualquier otro valor de la cantidad puede expresarse como un simple múltiplo de la unidad de medida. Por ejemplo, longitud es una cantidad; El metro es una unidad de longitud que representa una longitud predeterminada definida. Cuando decimos 10 metros (o 10 m), en realidad decimos 10 veces la longitud predeterminada definida llamada &quot;metro&quot;. (definición tomada de la ontología om)</rdfs:comment>
        <rdfs:isDefinedBy>http://www.wurvoc.org/vocabularies/om-1.8/</rdfs:isDefinedBy>
        <rdfs:label xml:lang="es">Unidad de Medida</rdfs:label>
        <rdfs:label xml:lang="en">Unit of Measure</rdfs:label>
    </owl:Class>
    


    <!-- 
    ///////////////////////////////////////////////////////////////////////////////////////
    //
    // Individuals
    //
    ///////////////////////////////////////////////////////////////////////////////////////
     -->

    


    <!-- http://dbpedia.org/resource/Decibel -->

    <owl:NamedIndividual rdf:about="http://dbpedia.org/resource/Decibel">
        <rdf:type rdf:resource="http://www.wurvoc.org/vocabularies/om-1.8/Unit_of_measure"/>
    </owl:NamedIndividual>
    


    <!-- http://vocab.linkeddata.es/datosabiertos/def/medio-ambiente/contaminacion-acustica#ClaseI -->

    <owl:NamedIndividual rdf:about="http://vocab.linkeddata.es/datosabiertos/def/medio-ambiente/contaminacion-acustica#ClaseI">
        <rdf:type rdf:resource="http://www.w3.org/2004/02/skos/core#Concept"/>
        <rdfs:comment xml:lang="es">Sensor que cumple las características de precisión más restrictivas definidas en la normativa IEC. Esta clase de sensores tiene menores márgenes de tolerancia en su rango de medida. Los instrumentos de Clase I se especifican dentro del rango de temperaturas del aire desde -10 ºC  hasta  +50 ºC.</rdfs:comment>
        <rdfs:label xml:lang="es">Clase I</rdfs:label>
        <rdfs:seeAlso xml:lang="es">Norma IEC 61672-1:2013</rdfs:seeAlso>
    </owl:NamedIndividual>
    


    <!-- http://vocab.linkeddata.es/datosabiertos/def/medio-ambiente/contaminacion-acustica#ClaseII -->

    <owl:NamedIndividual rdf:about="http://vocab.linkeddata.es/datosabiertos/def/medio-ambiente/contaminacion-acustica#ClaseII">
        <rdf:type rdf:resource="http://www.w3.org/2004/02/skos/core#Concept"/>
        <rdfs:comment xml:lang="es">Sensor que cumple las características de precisión menos restrictivas definidas en la normativa IEC. Esta clase de sensores tiene mayores márgenes de tolerancia en su rango de medida. Los instrumentos de Clase II se especifican dentro del rango de temperaturas del aire desde 0 ºC  hasta  +40 ºC.</rdfs:comment>
        <rdfs:label xml:lang="es">Clase II</rdfs:label>
        <rdfs:seeAlso xml:lang="es">Norma IEC 61672-1:2013</rdfs:seeAlso>
    </owl:NamedIndividual>
    


    <!-- http://vocab.linkeddata.es/datosabiertos/def/medio-ambiente/contaminacion-acustica#L01 -->

    <owl:NamedIndividual rdf:about="http://vocab.linkeddata.es/datosabiertos/def/medio-ambiente/contaminacion-acustica#L01">
        <rdf:type rdf:resource="http://vocab.linkeddata.es/datosabiertos/def/medio-ambiente/contaminacion-acustica#PercentilNoiseLevel"/>
        <rdfs:comment xml:lang="es">Nivel de ruido que se sobrepasa durante el 1% del tiempo de observación.</rdfs:comment>
        <rdfs:label xml:lang="es">Nivel de ruido sobre el 1%</rdfs:label>
    </owl:NamedIndividual>
    


    <!-- http://vocab.linkeddata.es/datosabiertos/def/medio-ambiente/contaminacion-acustica#L10 -->

    <owl:NamedIndividual rdf:about="http://vocab.linkeddata.es/datosabiertos/def/medio-ambiente/contaminacion-acustica#L10">
        <rdf:type rdf:resource="http://vocab.linkeddata.es/datosabiertos/def/medio-ambiente/contaminacion-acustica#PercentilNoiseLevel"/>
        <rdfs:comment xml:lang="es">Nivel de ruido que se sobrepasa durante el 10% del tiempo de observación</rdfs:comment>
        <rdfs:label xml:lang="es">Nivel de ruido sobre el 10%</rdfs:label>
    </owl:NamedIndividual>
    


    <!-- http://vocab.linkeddata.es/datosabiertos/def/medio-ambiente/contaminacion-acustica#L50 -->

    <owl:NamedIndividual rdf:about="http://vocab.linkeddata.es/datosabiertos/def/medio-ambiente/contaminacion-acustica#L50">
        <rdf:type rdf:resource="http://vocab.linkeddata.es/datosabiertos/def/medio-ambiente/contaminacion-acustica#PercentilNoiseLevel"/>
        <rdfs:comment xml:lang="es">Nivel de ruido que se sobrepasa durante el 50% del tiempo de observación</rdfs:comment>
        <rdfs:label xml:lang="es">Nivel de ruido sobre el 50%</rdfs:label>
    </owl:NamedIndividual>
    


    <!-- http://vocab.linkeddata.es/datosabiertos/def/medio-ambiente/contaminacion-acustica#L90 -->

    <owl:NamedIndividual rdf:about="http://vocab.linkeddata.es/datosabiertos/def/medio-ambiente/contaminacion-acustica#L90">
        <rdf:type rdf:resource="http://vocab.linkeddata.es/datosabiertos/def/medio-ambiente/contaminacion-acustica#PercentilNoiseLevel"/>
        <rdfs:comment xml:lang="es">Nivel de ruido que se sobrepasa durante el 90% del tiempo de observación</rdfs:comment>
        <rdfs:label xml:lang="es">Nivel de ruido sobre el 90%</rdfs:label>
    </owl:NamedIndividual>
    


    <!-- http://vocab.linkeddata.es/datosabiertos/def/medio-ambiente/contaminacion-acustica#L99 -->

    <owl:NamedIndividual rdf:about="http://vocab.linkeddata.es/datosabiertos/def/medio-ambiente/contaminacion-acustica#L99">
        <rdf:type rdf:resource="http://vocab.linkeddata.es/datosabiertos/def/medio-ambiente/contaminacion-acustica#PercentilNoiseLevel"/>
        <rdfs:comment xml:lang="es">Nivel de ruido que se sobrepasa durante el 99% del tiempo de observación</rdfs:comment>
        <rdfs:label xml:lang="es">Nivel de ruido sobre el 99%</rdfs:label>
    </owl:NamedIndividual>
    


    <!-- http://vocab.linkeddata.es/datosabiertos/def/medio-ambiente/contaminacion-acustica#Ld -->

    <owl:NamedIndividual rdf:about="http://vocab.linkeddata.es/datosabiertos/def/medio-ambiente/contaminacion-acustica#Ld">
        <rdf:type rdf:resource="http://vocab.linkeddata.es/datosabiertos/def/medio-ambiente/contaminacion-acustica#AverageNoiseLevel"/>
        <rdfs:comment xml:lang="es">Nivel de ruido día que se define como el valor medio del sonido medido en el periodo diurno (7-19 horas)</rdfs:comment>
        <rdfs:label xml:lang="en">Day noise level</rdfs:label>
        <rdfs:label xml:lang="es">Nivel de ruido día</rdfs:label>
        <rdfs:seeAlso xml:lang="es">ISO 1996-2: 1987</rdfs:seeAlso>
    </owl:NamedIndividual>
    


    <!-- http://vocab.linkeddata.es/datosabiertos/def/medio-ambiente/contaminacion-acustica#Lden -->

    <owl:NamedIndividual rdf:about="http://vocab.linkeddata.es/datosabiertos/def/medio-ambiente/contaminacion-acustica#Lden">
        <rdf:type rdf:resource="http://vocab.linkeddata.es/datosabiertos/def/medio-ambiente/contaminacion-acustica#AverageNoiseLevel"/>
        <rdfs:comment xml:lang="es">Valor medio del sonido medido dentro de un período de 24 horas, en el que se incluyen los valores obtenidos en Ld, Le, Ln.</rdfs:comment>
        <rdfs:label xml:lang="en">Day-evening-night noise level</rdfs:label>
        <rdfs:label xml:lang="es">Nivel de ruido día-tarde-noche</rdfs:label>
        <rdfs:seeAlso xml:lang="es">ISO 1996-2: 1987</rdfs:seeAlso>
    </owl:NamedIndividual>
    


    <!-- http://vocab.linkeddata.es/datosabiertos/def/medio-ambiente/contaminacion-acustica#Le -->

    <owl:NamedIndividual rdf:about="http://vocab.linkeddata.es/datosabiertos/def/medio-ambiente/contaminacion-acustica#Le">
        <rdf:type rdf:resource="http://vocab.linkeddata.es/datosabiertos/def/medio-ambiente/contaminacion-acustica#AverageNoiseLevel"/>
        <rdfs:comment xml:lang="es">Valor medio del  sonido medido en el periodo vespertino (19 - 23 horas)</rdfs:comment>
        <rdfs:label xml:lang="en">Evening noise level</rdfs:label>
        <rdfs:label xml:lang="es">Nivel de ruido vespertino</rdfs:label>
        <rdfs:seeAlso xml:lang="es">ISO 1996-2: 1987</rdfs:seeAlso>
    </owl:NamedIndividual>
    


    <!-- http://vocab.linkeddata.es/datosabiertos/def/medio-ambiente/contaminacion-acustica#Ln -->

    <owl:NamedIndividual rdf:about="http://vocab.linkeddata.es/datosabiertos/def/medio-ambiente/contaminacion-acustica#Ln">
        <rdf:type rdf:resource="http://vocab.linkeddata.es/datosabiertos/def/medio-ambiente/contaminacion-acustica#AverageNoiseLevel"/>
        <rdfs:comment xml:lang="es">Valor medio del sonido medido en el periodo nocturno (23 - 7 horas)</rdfs:comment>
        <rdfs:label xml:lang="en">Night noise level</rdfs:label>
        <rdfs:label xml:lang="es">Nivel de ruido de noche</rdfs:label>
        <rdfs:seeAlso xml:lang="es">ISO 1996-2: 1987</rdfs:seeAlso>
    </owl:NamedIndividual>
    


    <!-- http://vocab.linkeddata.es/datosabiertos/def/medio-ambiente/contaminacion-acustica#PonderacionA -->

    <owl:NamedIndividual rdf:about="http://vocab.linkeddata.es/datosabiertos/def/medio-ambiente/contaminacion-acustica#PonderacionA">
        <rdf:type rdf:resource="http://vocab.linkeddata.es/datosabiertos/def/medio-ambiente/contaminacion-acustica#Weighting"/>
        <rdf:type rdf:resource="http://www.w3.org/2004/02/skos/core#Concept"/>
        <rdfs:comment xml:lang="es">Ponderación más habitual en acústica ambiental. Se utiliza para ajustar los niveles de ruido a cómo los percibe el oido humano.</rdfs:comment>
        <rdfs:label xml:lang="es">Ponderación A</rdfs:label>
        <rdfs:seeAlso xml:lang="es">Norma IEC 61672:2003</rdfs:seeAlso>
    </owl:NamedIndividual>
    


    <!-- http://vocab.linkeddata.es/datosabiertos/def/medio-ambiente/contaminacion-acustica#PonderacionC -->

    <owl:NamedIndividual rdf:about="http://vocab.linkeddata.es/datosabiertos/def/medio-ambiente/contaminacion-acustica#PonderacionC">
        <rdf:type rdf:resource="http://vocab.linkeddata.es/datosabiertos/def/medio-ambiente/contaminacion-acustica#Weighting"/>
        <rdf:type rdf:resource="http://www.w3.org/2004/02/skos/core#Concept"/>
        <rdfs:comment xml:lang="es">Ponderación que se utiliza para evaluar altos niveles de ruido.</rdfs:comment>
        <rdfs:label xml:lang="es">Ponderación C</rdfs:label>
        <rdfs:seeAlso xml:lang="es">Norma IEC 61672:2003</rdfs:seeAlso>
    </owl:NamedIndividual>
    


    <!-- http://vocab.linkeddata.es/datosabiertos/def/medio-ambiente/contaminacion-acustica#PonderacionZ -->

    <owl:NamedIndividual rdf:about="http://vocab.linkeddata.es/datosabiertos/def/medio-ambiente/contaminacion-acustica#PonderacionZ">
        <rdf:type rdf:resource="http://vocab.linkeddata.es/datosabiertos/def/medio-ambiente/contaminacion-acustica#Weighting"/>
        <rdf:type rdf:resource="http://www.w3.org/2004/02/skos/core#Concept"/>
        <rdfs:comment xml:lang="es">Representa el hecho de no aplicar ningún tipo de ponderación frecuencial a las ondas sonoras captadas por el sensor de ruido. Se captan tal y como son.</rdfs:comment>
        <rdfs:label xml:lang="es">Ponderación Z</rdfs:label>
        <rdfs:seeAlso xml:lang="es">Norma IEC 61672:2003</rdfs:seeAlso>
    </owl:NamedIndividual>
    


    <!-- 
    ///////////////////////////////////////////////////////////////////////////////////////
    //
    // Annotations
    //
    ///////////////////////////////////////////////////////////////////////////////////////
     -->

    <rdf:Description rdf:about="http://www.w3.org/2003/01/geo/wgs84_pos#">
        <dc:date>$Date: 2009/04/20 15:00:30 $</dc:date>
        <rdfs:label>geo</rdfs:label>
        <dc:description>A vocabulary for representing latitude, longitude and 
 altitude information in the WGS84 geodetic reference datum. 
 Version $Id: wgs84_pos.rdf,v 1.22 2009/04/20 15:00:30 timbl Exp $. See http://www.w3.org/2003/01/geo/ for more details.</dc:description>
        <rdfs:comment>
Recent changes to this namespace:
$Log: wgs84_pos.rdf,v $
Revision 1.22  2009/04/20 15:00:30  timbl
Remove the time bits which have been deal with elsewhere eg in iCal.

Revision 1.21  2009/04/20 12:52:47  timbl
try again

Revision 1.20  2009/04/20 12:42:11  timbl
Add Event (edited ages ago and never checked in), and location (following discussion http://chatlogs.planetrdf.com/swig/2009-04-20#T12-36-09)

Revision 1.19  2009/04/20 12:36:31  timbl
Add Event (edited ages ago and never checked in), and location (following discussion http://chatlogs.planetrdf.com/swig/2009-04-20#T12-36-09)

Revision 1.18  2006/02/01 22:01:04  danbri
Clarified that lat and long are decimal degrees, and that alt is decimal metres about local reference ellipsoid

Revision 1.17  2004/02/06 17:38:12  danbri
Fixed a bad commit screwup

Revision 1.15  2003/04/19 11:24:08  danbri
Fixed the typo even more.

Revision 1.14  2003/04/19 11:16:56  danbri
fixed a typo

Revision 1.13  2003/02/19 22:27:27  connolly
relaxed domain constraints on lat/long/alt from Point to SpatialThing

Revision 1.12  2003/01/12 01:41:41  danbri
Trying local copy of XSLT doc.

Revision 1.11  2003/01/12 01:20:18  danbri
added a link to morten&apos;s xslt rdfs viewer.

Revision 1.10  2003/01/11 18:56:49  danbri
Removed datatype range from lat and long properties, since they would
have required each occurance of the property to mention the datatype.

Revision 1.9  2003/01/11 11:41:31  danbri
Another typo; repaired rdfs:Property to rdf:Property x4

Revision 1.8  2003/01/11 11:05:02  danbri
Added an rdfs:range for each lat/long/alt property,
http://www.w3.org/2001/XMLSchema#float

Revision 1.7  2003/01/10 20:25:16  danbri
Longer rdfs:comment for Point, trying to be Earth-centric and neutral about
coordinate system(s) at the same time. Feedback welcomed.

Revision 1.6  2003/01/10 20:18:30  danbri
Added CVS log comments into the RDF/XML as an rdfs:comment property of the
vocabulary. Note that this is not common practice (but seems both harmless
and potentially useful).


revision 1.5
date: 2003/01/10 20:14:31;  author: danbri;  state: Exp;  lines: +16 -5
Updated schema:
Added a dc:date, added url for more info. Changed the rdfs:label of the
namespace from gp to geo. Added a class Point, set as the rdfs:domain of
each property. Added XML comment on the lat_long property suggesting that
we might not need it (based on #rdfig commentary from implementors).

revision 1.4
date: 2003/01/10 20:01:07;  author: danbri;  state: Exp;  lines: +6 -5
Fixed typo; several rdfs:about attributes are now rdf:about. Thanks to MortenF in
#rdfig for catching this error.

revision 1.3
date: 2003/01/10 11:59:03;  author: danbri;  state: Exp;  lines: +4 -3
fixed buglet in vocab, added more wgs links

revision 1.2
date: 2003/01/10 11:01:11;  author: danbri;  state: Exp;  lines: +4 -4
Removed alt from the as-a-flat-string property, and switched from
space separated to comma separated.

revision 1.1
date: 2003/01/10 10:53:23;  author: danbri;  state: Exp;
basic geo vocab

</rdfs:comment>
        <dc:title>WGS84 Geo Positioning: an RDF vocabulary</dc:title>
    </rdf:Description>
    <rdf:Description rdf:about="http://www.w3.org/2003/01/geo/wgs84_pos#lat_long">
        <rdfs:comment>A comma-separated representation of a latitude, longitude coordinate.</rdfs:comment>
        <rdfs:label>lat/long</rdfs:label>
    </rdf:Description>
    <rdf:Description rdf:about="http://www.w3.org/2003/01/geo/wgs84_pos#location">
        <rdfs:label>location</rdfs:label>
        <rdfs:comment>The relation between something and the point, 
 or other geometrical thing in space, where it is.  For example, the realtionship between
 a radio tower and a Point with a given lat and long.
 Or a relationship between a park and its outline as a closed arc of points, or a road and
 its location as a arc (a sequence of points).
 Clearly in practice there will be limit to the accuracy of any such statement, but one would expect
 an accuracy appropriate for the size of the object and uses such as mapping .
 </rdfs:comment>
    </rdf:Description>
</rdf:RDF>



<!-- Generated by the OWL API (version 4.2.8.20170104-2310) https://github.com/owlcs/owlapi -->

